Examples.v
@@ -1,0 +1,355 @@
+(** * Examples. *)
+(** ** Example 1 from Section 3. *)
+Require Import Bool.
+
+Record state :=
+{ time : bool
+; high : bool
+; password : bool
+; query : bool
+; result : bool
+}.
+
+(** The step function of the system *)
+Definition step (s: state) : state :=
+if time s
+then s
+else
+{| time := true;
+   high := high s;
+   password := password s;
+   query := query s;
+   result := if bool_dec (password s) (query s)
+            then negb (result s)
+            else result s
+|}.
+
+(** The relation that describes the execution of the system. *)
+Definition exec : relation state :=
+  fun s1 s2 => s2 = s1 \/ s2 = step s1.
+
+Lemma exec_refl : forall s, exec s s.
+Proof.
+intro s. left. reflexivity.
+Qed.
+
+Definition password_checker : sys state :=
+  {| next := exec; next_refl := exec_refl |}.
+
+(** The observation that the observer is interested in. *)
+Definition R : relation state :=
+  fun s s' =>
+    time s = time s' /\ query s = query s' /\ result s = result s'.
+
+Instance R_Equivalence : Equivalence R.
+Proof.
+unfold R. constructor.
+* intro s. intuition.
+* intros s1 s2 H. intuition.
+* intros s1 s2 s3 H12 H23. simpl in *. intuition; eauto.
+Qed.
+Hint Resolve R_Equivalence.
+
+(** For the following lemma, it is crucial that password and query
+    are booleans. *)
+Lemma time_false_R_step_password :
+  forall s1 s2 : state,
+    time s1 = false ->
+    R s1 s2 ->
+    R (step s1) (step s2) ->
+    password s1 = password s2.
+Proof.
+intros s1 s2 Hfalse H H'.
+destruct H as [Ht [Hq Hr]].
+unfold step in H'.
+rewrite <- Ht in H'. clear Ht.
+rewrite <- Hq in H'. clear Hq.
+rewrite <- Hr in H'. clear Hr.
+rewrite Hfalse in H'. clear Hfalse.
+destruct H' as [Ht [Hq Hr]]. simpl in *.
+clear Ht Hq.
+destruct (bool_dec (password s1) (query s1));
+  destruct (bool_dec (password s2) (query s1)).
+* congruence.
+* exfalso. destruct (result s1); simpl in Hr; congruence.
+* exfalso. destruct (result s1); simpl in Hr; congruence.
+* destruct (query s1); destruct (password s1);
+  destruct (password s2); congruence.
+Qed.
+
+Lemma step_time_false_neq :
+  forall s,
+    time s = false ->
+    s <> step s.
+Proof.
+intros s H. unfold step.
+destruct s as [t h p q r]. simpl in *.
+subst t.
+congruence.
+Qed.
+
+Lemma step_time_true_eq :
+  forall s,
+    time s = true ->
+    s = step s.
+Proof.
+intros s H. unfold step.
+destruct s as [t h p q r]. simpl in *.
+subst t.
+reflexivity.
+Qed.
+
+Lemma R_step_time_false :
+  forall s s',
+    R s s' ->
+    time s = false ->
+    (time s = false -> password s = password s') ->
+    R (step s) (step s').
+Proof.
+intros s s' HR Hfalse Hpassword.
+destruct s  as [t  h  p  q  r].
+destruct s' as [t' h' p' q' r'].
+unfold step in *. simpl in *.
+subst t.
+destruct HR as [Htime [Hquery Hresult]].
+simpl in *.
+rewrite <- Htime.
+deep_splits; trivial.
+specialize (Hpassword eq_refl). subst. reflexivity.
+Qed.
+
+Lemma time_false_not_R_step :
+  forall s,
+    time s = false ->
+    ~ R s (step s).
+Proof.
+intros s Hfalse HR.
+unfold step in *. rewrite Hfalse in HR.
+destruct s as [t h p q r].
+destruct HR as [Ht [Hq Hr]].
+simpl in *.
+congruence.
+Qed.
+
+Lemma step_projection :
+  forall s, step s = step (step s).
+Proof.
+intros [t h p q r].
+destruct t; unfold step; simpl.
++ reflexivity.
++ f_equal.
+Qed.
+
+Definition trace_step (s : state) : trace password_checker.
+Proof.
+refine (trace_cons s (trace_one password_checker (step s)) _).
+* right. reflexivity.
+Defined.
+
+(** The traces of password_checker are of two possible kinds. *)
+Lemma stutter_password_checker (R: relation state) {E: Equivalence R}:
+  forall t : trace password_checker,
+    stutter_equiv
+      (view R t)
+      (view R (trace_one password_checker (hd t)))
+    \/ stutter_equiv
+         (view R t)
+         (view R (trace_step (hd t))).
+Proof.
+intros [l Hl]. induction l.
+* destruct Hl.
+* destruct l as [| b l].
+  - clear IHl. left. reflexivity.
+  - simpl. unfold hd in IHl. destruct Hl as [Hab Hbl].
+    specialize (IHl Hbl). destruct IHl as [IHl | IHl].
+    + { unfold view in IHl. simpl in IHl. destruct Hab as [Hab | Hab]; subst b.
+        * left. apply stutter_left. assumption.
+        * right. apply stutter_same. assumption.
+      }
+    + {  unfold view in IHl. simpl in IHl. destruct Hab as [Hab | Hab]; subst b.
+        * right. apply stutter_left. assumption.
+        * right. apply stutter_same.
+          transitivity (view R (trace_step (step a))).
+          + assumption.
+          + unfold trace_step. unfold view. simpl. rewrite <- step_projection.
+            apply stutter_left. reflexivity.
+      }
+Qed.
+
+Lemma time_false_obs_password :
+  forall s s': state,
+    obs_eq password_checker R s s' ->
+    time s = false ->
+    R s s' ->
+    password s = password s'.
+Proof.
+intros s s' Hobs Hfalse HR.
+apply time_false_R_step_password; trivial.
+destruct s  as [t  h  p  q  r].
+destruct s' as [t' h' p' q' r'].
+destruct HR as [Htime [Hquery Hresult]].
+simpl in *. subst.
+rewrite <- Htime in *. clear Htime. unfold step. simpl.
+deep_splits.
+simpl. destruct (bool_dec p p').
+* subst. reflexivity.
+* exfalso. apply n. clear n.
+  pose (s := {|
+              time := false;
+              high := h;
+              password := p;
+              query := q';
+              result := r' |}). fold s in Hobs.
+  pose (s' := {|
+               time := false;
+               high := h';
+               password := p';
+               query := q';
+               result := r' |}). fold s' in Hobs.
+  destruct Hobs as [Hss' Hs's].
+  assert (is_trace password_checker (s :: step s :: nil)) as Htrace.
+  { split; auto. right; reflexivity. }
+  pose (t := exist _ _ Htrace).
+  specialize (Hss' (view R t)).
+  destruct Hss' as [v' [[t0' [Hv' Ht0's']] Htt0']].
+  { exists t. split; reflexivity. }
+  subst v'.
+  assert (In (step s') (proj1_sig t0')).
+  { destruct (stutter_password_checker R t0') as [H | H].
+    * exfalso.
+      eapply (time_false_not_R_step s); trivial.
+      assert (forall a, In a (proj1_sig t) -> R a (hd t0')) as Haux.
+      { intros a Ha.
+        assert (In (R a) (view R t)). { apply in_map. assumption. }
+        assert (In (R a) (view R (trace_one password_checker (hd t0')))) as HR.
+        { apply (stutter_equiv_in (view R t)); trivial.
+          transitivity (view R t0'); trivial. }
+        destruct HR as [HR | HR].
+        + rewrite <- HR. apply class_refl.
+        + exfalso. simpl in HR. assumption.
+      }
+      transitivity (hd t0').
+      + apply Haux. unfold t. simpl. eauto.
+      + symmetry. apply Haux. unfold t. simpl. eauto.
+    * destruct t0' as [[| a0 l0] Hl0]; [destruct Hl0 |].
+      simpl in H. simpl proj1_sig. compute in Ht0's'. fold s' in Ht0's'.
+      subst.
+      apply (stutter_equiv_in (proj1_sig (trace_step s'))).
+      + symmetry. assumption.
+      + right. simpl. eauto.
+  }
+  assert (R (step s') s \/ R (step s') (step s)) as [? | ?].
+  { destruct Htt0' as [Htt0' Ht0't].
+    destruct (included_view_R _ _ _ Ht0't _ H) as [s1 [Hs1 Hs's1]].
+    destruct Hs1.
+    + subst s1. eauto.
+    + destruct H0.
+      - subst s1. eauto.
+      - destruct H0.
+  }
+  + destruct H0 as [H0 _].
+    unfold s' in H0; unfold step in H0; simpl in H0. congruence.
+  + destruct H0 as [_ [ _ H0]].
+    unfold s' in H0; unfold step in H0; simpl in H0.
+    destruct (bool_dec p' q'); destruct (bool_dec p q').
+    - congruence.
+    - destruct r'; simpl in H0; congruence.
+    - destruct r'; simpl in H0; congruence.
+    - destruct p; destruct p'; destruct q'; try congruence.
+Qed.
+
+Lemma R_included_obs:
+  forall (s s': state),
+    R s s' ->
+    R (step s) (step s') ->
+    set_included (set_equiv stutter)
+                 (obs_from s password_checker R)
+                 (obs_from s' password_checker R).
+Proof.
+intros s s' HR HR'.
+intros v [t [Hv Hts]]. subst v.
+destruct (stutter_password_checker t) as [H | H].
+- destruct t as [[| a l] Hl]; [destruct Hl |].
+  compute in Hts. subst a. simpl_ctx.
+  apply stutter_one_stutter_view; trivial.
+- destruct t as [[| a l] Hl]; [destruct Hl |].
+  compute in Hts. subst a. simpl_ctx.
+  { case_eq (time s); intro Htime'.
+    * pose proof (step_time_true_eq _ Htime') as Hstep.
+      rewrite <- Hstep in H. clear Hstep.
+      assert (stutter_equiv (s :: l) (s :: nil)) as H'.
+      { transitivity (s :: s :: nil). assumption. auto. }
+      clear H. apply stutter_one_stutter_view; trivial.
+    * pose proof (step_time_false_neq _ Htime') as Hstep.
+      destruct (stutter_two_inv _ _ _ Hstep H) as [n1 [n2 Heq]].
+      clear Hstep.
+      pose (l' :=
+              s' :: repeat s' n1
+              ++ step s' :: repeat (step s') n2).
+      assert (is_trace password_checker l') as Htrace'.
+      { apply is_trace_repeat_two. right; reflexivity. }
+      pose (t' := exist _ _ Htrace').
+      exists (view R t'). split.
+      + exists t'. split; reflexivity.
+      + split.
+        - intros t0 Ht0. exists t0.
+          { split.
+            * transitivity (exist _ _ Hl); trivial.
+              symmetry.
+              unfold t'. simpl_view. split; trivial.
+              inversion Heq; subst.
+              apply repeat_two_same_view; trivial.
+            * reflexivity.
+          }
+        - intros t0 Ht0. exists t0.
+          { split.
+            * transitivity t'; trivial.
+              unfold t'. simpl_view. split; trivial.
+              inversion Heq; subst.
+              apply repeat_two_same_view; trivial.
+            * reflexivity.
+          }
+  }
+Qed.
+
+Lemma R_time_included_obs:
+  forall (s s': state),
+    R s s' ->
+    (time s = false -> password s = password s') ->
+    set_included (set_equiv stutter)
+                 (obs_from s password_checker R)
+                 (obs_from s' password_checker R).
+Proof.
+intros s s' HR Htime.
+apply R_included_obs; trivial.
+case_eq (time s); intro H.
+* repeat rewrite <- step_time_true_eq; trivial.
+  destruct HR as [Ht _]. congruence.
+* apply R_step_time_false; trivial.
+Qed.
+
+Lemma password_checker_obs_eq_iff :
+  forall s s',
+    obs_eq password_checker R s s'
+    <->
+    (time s = time s' /\ query s = query s' /\ result s = result s'
+     /\ (time s = false -> password s = password s')).
+Proof.
+intros s s'. split.
+* intro Hobs_eq.
+  cut (R s s' /\ (R s s' -> time s = false -> password s = password s')).
+  + intros [? ?]. unfold R in *. intuition.
+  + split.
+    - apply (obs_eq_R _ _ Hobs_eq).
+    - intros Hr Hfalse. apply time_false_obs_password; auto.
+* intro H.
+  assert (R s s' /\ (time s = false -> password s = password s'))
+    as [HR Htime]. { unfold R. intuition. }
+  clear H. split.
+  + apply R_time_included_obs; trivial.
+  + apply R_time_included_obs; trivial.
+    - symmetry. trivial.
+    - intro H. symmetry. apply Htime. destruct HR as [Ht _]. congruence.
+Qed.
+
+(** TODO: rest of the examples. *)
