Makefile
@@ -1,8 +1,9 @@
 MODULES := MyTactics \
-	   SetPredicates \
+	   EquivClass SetPredicates \
 	   Lattice Kleene \
            NatLattice SetLattice RelLattice PERLattice ERLattice \
-           Stutter View Robustness
+           Stutter View Robustness \
+           Examples
 
 VS 	:= $(MODULES:%=%.v)
 
